\documentclass[11pt, sakura, night, 0.5in]{hw}

\def\course{MAT159}
\def\headername{Week 10}
\def\logo{clsfiles/qunwang}

\usepackage{mathtools}

\begin{document}

\coverpage

\tbf{\underline{Week 10}}

\tbf{Review.}

If $f_n$ is a \underline{sequence} of functions \[f_n: D\subseteq \R\to\R,\] and $f$ is a function \[f: D\subseteq \R\to\R.\]

Convergence:
\begin{itemize}
    \item Pointwise $f_n\to f$
    \item Uniform $f_n\rightrightarrows f$
\end{itemize}

In practice, this type of problem comes often from the mission of represent $f$ by series (usually a basis of an infinite dimensional space)

\tbf{Example.}

\begin{itemize}
    \item Polynomials \[f \stackrel{?}{=} \sum_{n=0}^\infty a_n x^n\quad f_n = \sum_{n=0}^m a_n x^n.\]
    \item Trigonometric \[f\stackrel{?}{=} \sum_{n=0}^\infty a_n \sin(nx)\quad f_n=\sum_{n=0}^m a_n\sin(nx).\]
\end{itemize}

Assume that one have a function series \[\sum_{n=1}^\infty u_n(x)\quad u_n:D\subseteq\R\to\R.\]

Now if we want to study the partial sum, \[f_n:\sum_{n=1}^m u_n\quad \T{series}\to\T{sequence}\]

\[f_m: \underbrace{(f_n-f_{n-1})}_{u_n} + \underbrace{(f_{n+1}-f_{n-2})}_{u_{n-1}} +\cdots+\underbrace{(f_2-f_1)}_{u_2}+\underbrace{(f_1-f_0)}_{u_1}+\underbrace{f_0}_{u_0}\]

\[f_m:\sum_{j=1}^n u_j\quad\T{sequence}\to\T{series}\]

\newt[Recall Cauchy Criterion]{1}{

\(\ds\sum_{n=1}^\infty u_n(x)\quad \T{converges to $f$ if}\)

\[\forall x\in D. \forall \ep>0.\exists N_0\in\N\st\forall m>n>N_0, \abs{\sum_{n+1}^m u_j(x)}<\ep.\]
}

\newr{
    If the above choice of $N_0$ is independent of $x\in D$, then the convergence is \underline{uniform}.
}

\newt[Abel Identity]{2}{
    \[\sum_{i=n+1}^m a_ib_i\]

    By change of variable: \[B_k = \sum_{i=1}^k b_i,\quad B_0=0,\]

    The above is equal to \begin{align*}
        \sum_{i=n+1}^m a_ib_i=\sum_{i=1}^m a_i(B_i-B_{i-1})&=a_1B_1+a_2(B_2-B_1)+a_3(B_3-B_2)+\cdots+a_m(B_m-B_{m-1})\\
        &=(a_1-a_2)B_1+(a_2-a_3)B_2+(a_3-a_4)B_3+\cdots+(a_{m-1}-a_m)B_{m-1}+a_mB_m\\
        &=a_mB_m-\sum_{i=1}^{m-1}(a_{i+1}-a_i)B_i.
    \end{align*}
}

\newr{
    This is just an \underline{integration by parts} (discrete version).

    ``Morally speaking''

    \[a_i=f(x_i)\quad b_i=g(x_i)\quad B_i\approx \int_a^{x_i}g(x_i)\D x_i = G(x_i)\]

    \[\sum a_i b_i\approx \int f(x)g(x)\D x=\int f(x)\D G(x) = f(x)G(x)\bigg|_{a}^b - \int_a^b G(x)\D f(x)\approx a_mB_m-\sum_{i=1}^{m-1}(a_{i+1}-a_i)B_i.\]
}

Now, remember what you want to control. Back to analysis of convergence. Given a constant seris $\ds\sum_{i=1}^m a_i b_i$. By Cauchy we need to have \[\abs{\sum_{i=n+1}^m a_ib_i}\over{m,n\to\infty}{\longrightarrow}0\]

According to Abel identity, \begin{align*}
    \sum_{i=n+1}^m a_ib_i&=a_{n+1}b_{n+1}+a_{n+2}b_{n+2}+\cdots+a_mb_m\\
    &=a_{n+1}(B_{n+1}-B_n)+a_{n+2}(B_{n+1}-B_{n+2})+\cdots+a_m(B_m-B_{m-1})\\
    &=\abs{a_mB_m-\sum_{i=n}^{m-1}(a_{i+1}-a_i)B_i-a_nB_n}
    \alt{Observe that $|B_n|\le L$,}
    R_{m,n}&\le \abs{a_mB_m-a_nB_m +a_nB_m-a_nB_n-\sum_{i=n}^{m-1}(a_{i+1}-a_i)B_i}\\
    &\le \abs{a_m-a_n}L+|a_n|\abs{B_m-B_n} + L\sum_{i=n}^{m-1}\abs{a_{i+1}-a_i}
    \alt{Since $a_n$ is monotonic (increasing or decreasing)}
    R_{m,n}&\le |a_m-a_n|L+|a_n||B_m-B_n|+L|a_m-a_n|\\
    \alt{How to force $R_{m,n}\to0$?}
    \alt{\underline{\tbf{Combo 1}} $B_n\to0$ and $a_n$ bounded. We can see that $R_{m,n}\to0$ since $a_n$ converges. This is called the Abel Test.}
    \alt{\underline{\tbf{Combo 2}} $B_n$ bounded and $a_n\to0$. This is called the Dirichlet Test.}
\end{align*}

\neweg{
    \[\sum_{n=1}^\infty \underbrace{(-1)^{n+1}}_{B_n}\cd a_n\quad \T{$a_n$ is decreasing to 0}\]

    Since $B_n\in\{-1,1\}$, by dirichlet the series converges.
}

\newr{
    \[\sum_{i=1}^\infty a_i(x)b_i(x)\to f(x)\]

    We can solve the above using Abel / Dirichlet Test.

    \[\sum_{i=1}^\infty a_i(x)b_i(x)\rightrightarrows f(x)\]

    For the above, we can simply change the conditions to uniform, e.g. bounded to bounded uniformly, converge to converge uniformly.
}

\neweg{
    Let's consider \[\sum_{n=1}^{\infty}\frac{a_n}{n^x}\quad\T{$a_n$ is arbitrary}.\]

    If $a_n\is1$ then this is just the p-harmonic series, ez.

    If $\ds\sum_{n=1}^\infty \frac{a_n}{n^x}$ converges for some $x_0$. Then $\forall x>x_0, \ds\sum_{n=1}^\infty \frac{a_n}{n^{x}}=\sum_{n=1}^\infty\underbrace{\frac{a_n}{n^{x_0}}}_{\T{converge}}\cd\underbrace{\frac{1}{n^{x-x_0}}}_{\T{monotonic and bounded}}<\infty$ by Abel Test it converges.
}





\end{document}